Proved progress for wcbv reduction

erasure/theories/ErasureFunction.v
@@ -16,6 +16,7 @@ From MetaCoq.PCUIC Require Import PCUICAst PCUICAstUtils PCUICPrimitive
 From MetaCoq.SafeChecker Require Import PCUICErrors PCUICSafeReduce PCUICSafeRetyping.
 From MetaCoq.Erasure Require Import EAstUtils EArities Extract Prelim EDeps ErasureCorrectness.
 
+
 Local Open Scope string_scope.
 Set Asymmetric Patterns.
 Import MCMonadNotation.
@@ -1338,7 +1339,7 @@ Qed.
 Section firstorder.
 
 Context {Σ : global_env_ext}.
-Context {Σb : list (kername × list bool)}.
+Context {Σb : list (kername × (Instance.t -> list bool))}.
 
 Fixpoint plookup_env {A} (Σ : list (kername × A)) (kn : kername) {struct Σ} :
 option A :=
@@ -1346,7 +1347,7 @@ match Σ with
 | [] => None
 | d :: tl => if eq_kername kn d.1 then Some d.2 else plookup_env tl kn
 end. 
-
+(* 
 Definition zo_type (t : term) :=
   match (PCUICAstUtils.decompose_app t).1 with
   | tProd _ _ _ => false
@@ -1355,39 +1356,41 @@ Definition zo_type (t : term) :=
                            | Some l => nth i l false | None => false
                            end
   | _ => true
-  end.
+  end. *)
 
-Definition firstorder_params (t : term) :=
+Definition firstorder_type (t : term) :=
+  match (PCUICAstUtils.decompose_app t).1 with
+  | tInd (mkInd nm i) u => match (plookup_env Σb nm) with 
+                           | Some f => nth i (f u) false | None => true
+                           end
+  | _ => false
+  end.
+(* 
+Definition firstorder_type (t : term) :=
   match (PCUICAstUtils.decompose_app t).1 with
   | tInd (mkInd nm i) _ => match (plookup_env Σb nm) with 
                            | Some l => nth i l false | None => false
                            end
-  | _ => true
-  end.
+  | _ => false
+  end. *)
 
-Fixpoint firstorder_type (t : term) :=
-  match t with
-  | tProd _ t1 t2 => zo_type t2 && firstorder_type t2
-  | _ => true
-  end.
+Definition firstorder_con i u mind (c : constructor_body):=
+  forallb (fun '({| decl_body := b ; decl_type := t ; decl_name := n|}) => firstorder_type t) 
+    (subst_context (inds i u mind.(ind_bodies)) 0 (c.(cstr_args) ++ mind.(ind_params))@[u])%list.
 
-Definition firstorder_con (c : constructor_body) :=
-  forallb (fun '({| decl_body := b ; decl_type := t ; decl_name := n|}) => firstorder_type t) c.(cstr_args) &&
-  forallb (firstorder_params) c.(cstr_indices).
-
-Definition firstorder_oneind (ind : one_inductive_body) :=
-  forallb firstorder_con ind.(ind_ctors) && negb (Universe.is_level (ind_sort ind)).
+Definition firstorder_oneind i u mind (ind : one_inductive_body) :=
+  forallb (firstorder_con i u mind) ind.(ind_ctors) && negb (Universe.is_level (ind_sort ind)).
   
-Definition firstorder_mutind (mind : mutual_inductive_body) :=
-  if forallb (fun decl => firstorder_params decl.(decl_type)) mind.(ind_params) then
-  map firstorder_oneind mind.(ind_bodies)
-  else repeat false (length mind.(ind_bodies)).
+Definition firstorder_mutind i u (mind : mutual_inductive_body) :=
+  (* if forallb (fun decl => firstorder_type decl.(decl_type)) mind.(ind_params) then *)
+  map (firstorder_oneind i u mind) mind.(ind_bodies)
+  (* else repeat false (length mind.(ind_bodies)). *).
 
-Definition firstorder_ind (i : inductive) :=
+Definition firstorder_ind (i : inductive) u :=
   match lookup_env Σ.1 (inductive_mind i) with
   | Some (InductiveDecl mind) =>
       check_recursivity_kind Σ (inductive_mind i) Finite &&
-      nth (inductive_ind i) (firstorder_mutind mind) false
+      nth (inductive_ind i) (firstorder_mutind i.(inductive_mind) u mind) false
   | _ => false
   end.
 
@@ -1396,8 +1399,8 @@ End firstorder.
 Fixpoint firstorder_env' (Σ : global_env) Σb :=
   match Σ with
   | nil => Σb
-  | (nm, ConstantDecl _) :: Σ' => firstorder_env' Σ' ((nm, []) :: Σb) 
-  | (nm, InductiveDecl mind) :: Σ' => firstorder_env' Σ' ((nm, @firstorder_mutind Σb mind) :: Σb)
+  | (nm, ConstantDecl _) :: Σ' => firstorder_env' Σ' ((nm, fun _ => []) :: Σb) 
+  | (nm, InductiveDecl mind) :: Σ' => firstorder_env' Σ' ((nm, (fun u => @firstorder_mutind Σb nm u mind)) :: Σb)
   end.                            
 
 Definition firstorder_env Σ :=
@@ -1536,25 +1539,24 @@ Proof.
   induction H0; econstructor; eauto.
 Qed.
 
-Lemma firstorder_ind_propositional {Σ : global_env_ext} i mind oind :
+Lemma firstorder_ind_propositional {Σ : global_env_ext} i mind oind u :
   squash (wf_ext Σ) ->
   declared_inductive Σ i mind oind ->
-  @firstorder_ind Σ (firstorder_env Σ) i ->
+  @firstorder_ind Σ (firstorder_env Σ) i u ->
   isPropositional Σ i false.
 Proof.
   intros Hwf d. pose proof d as [d1 d2]. intros H. red in d1. unfold firstorder_ind in H.
   red. sq.
   unfold PCUICEnvironment.fst_ctx in *. rewrite d1 in H |- *.
-  solve_all. unfold firstorder_mutind in H0.
-  destruct forallb eqn:E.
-  - rewrite d2. eapply map_nth_error with (f := @firstorder_oneind (firstorder_env Σ)) in d2.
-    erewrite nth_nth_error in H0. rewrite d2 in H0.
-    unfold firstorder_oneind in H0. solve_all.
-    destruct (ind_sort oind) eqn:E2; inv H1. clear H3.
-    eapply PCUICInductives.declared_inductive_type in d.
-    rewrite d. rewrite E2.
-    now rewrite destArity_it_mkProd_or_LetIn.
-  - rewrite nth_repeat in H0. congruence.
+  solve_all.
+  unfold firstorder_mutind in H0.
+  rewrite d2. eapply map_nth_error with (f := @firstorder_oneind (firstorder_env Σ) (inductive_mind i) u mind) in d2.
+  erewrite nth_nth_error in H0. rewrite d2 in H0.
+  unfold firstorder_oneind in H0. solve_all.
+  destruct (ind_sort oind) eqn:E2; inv H1. clear H3.
+  eapply PCUICInductives.declared_inductive_type in d.
+  rewrite d. rewrite E2.
+  now rewrite destArity_it_mkProd_or_LetIn.
 Qed.
 
 Inductive firstorder_spine {cf} Σ (Γ : context) : term -> list term -> term -> Type :=
@@ -1570,26 +1572,225 @@ Inductive firstorder_spine {cf} Σ (Γ : context) : term -> list term -> term ->
     Σ ;;; Γ ⊢ ty ≤ tProd na (mkApps (tInd i u) args) B ->
     declared_inductive Σ i mind oind ->
     Σ ;;; Γ |- hd : (mkApps (tInd i u) args) ->
-    @firstorder_ind Σ (@firstorder_env Σ) i ->
+    @firstorder_ind Σ (@firstorder_env Σ) i u ->
     firstorder_spine Σ Γ (subst10 hd B) tl B' ->
     firstorder_spine Σ Γ ty (hd :: tl) B'.
 
-Lemma firstorder_args {Σ : global_env_ext} { Γ mind cbody i n ui args u pandi oind} :
-  declared_constructor Σ (i, n) mind oind cbody ->
-  PCUICArities.typing_spine Σ Γ (type_of_constructor mind cbody (i, n) ui) args (mkApps (tInd i u) pandi) ->
-  @firstorder_ind Σ (@firstorder_env Σ) i ->
-  firstorder_spine Σ Γ (type_of_constructor mind cbody (i, n) ui) args (mkApps (tInd i u) pandi).
+Inductive instantiated {Σ} (Γ : context) : term -> Type :=
+| instantiated_mkApps i u args : instantiated Γ (mkApps (tInd i u) args)
+| instantiated_tProd na B i u args : 
+  @firstorder_ind Σ (@firstorder_env Σ) i u ->
+    (forall x, Σ ;;; Γ |- x : mkApps (tInd i u) args -> instantiated Γ (subst10 x B)) ->
+    instantiated Γ (tProd na (mkApps (tInd i u) args) B).
+
+From MetaCoq Require Import PCUICArities PCUICSpine.
+
+Lemma typing_spine_arity_spine cf Σ Γ Δ args T' i u pars :
+    typing_spine Σ Γ (it_mkProd_or_LetIn Δ (mkApps (tInd i u) pars)) args T' ->
+    arity_spine Σ Γ (it_mkProd_or_LetIn Δ (mkApps (tInd i u) pars)) args T'.
 Proof.
+  intros H. revert args pars T' H.
+  induction Δ using PCUICInduction.ctx_length_rev_ind; intros args pars T' H.
+  - cbn. depelim H.
+    + econstructor; eauto.
+    + eapply PCUICCanonicity.invert_cumul_ind_prod in e. eauto.
+  - cbn. depelim H.
+    + econstructor; eauto.
+    + rewrite it_mkProd_or_LetIn_app in e, i0 |- *. cbn. destruct d as [name [body |] type]; cbn in *.
+      -- todo "let". 
+      -- eapply cumul_Prod_inv in e as []. econstructor.
+         ++ eapply type_equality. 3: eapply PCUICContextConversion.equality_eq_le; symmetry. all:eauto.
+            eapply isType_tProd in i0. eapply i0.
+         ++ rewrite /subst1 PCUICLiftSubst.subst_it_mkProd_or_LetIn. autorewrite with subst.
+            cbn. eapply X. len.
+            eapply typing_spine_strengthen. eauto. 
+            2:{ replace (it_mkProd_or_LetIn (subst_context [hd] 0 Γ0)
+            (mkApps (tInd i u) (map (subst [hd] (#|Γ0| + 0)) pars))) with ((PA.subst10 hd (it_mkProd_or_LetIn Γ0 (mkApps (tInd i u) pars)))).
+            2:{ rewrite /subst1 PCUICLiftSubst.subst_it_mkProd_or_LetIn. now autorewrite with subst. }   
+            eapply substitution0_equality. eauto. eauto.
+            }
+            replace (it_mkProd_or_LetIn (subst_context [hd] 0 Γ0)
+            (mkApps (tInd i u) (map (subst [hd] (#|Γ0| + 0)) pars))) with ((PA.subst10 hd (it_mkProd_or_LetIn Γ0 (mkApps (tInd i u) pars)))).
+            2:{ rewrite /subst1 PCUICLiftSubst.subst_it_mkProd_or_LetIn. now autorewrite with subst. }   
+            eapply isType_subst. eapply PCUICSubstitution.subslet_ass_tip. eauto.
+            eapply isType_context_equality. 
+            eapply isType_tProd in i0. eapply i0. econstructor. eapply typing_wf_local. eauto.
+            eapply isType_tProd in i1. eapply i1. econstructor. eapply context_equality_refl.
+            todo "search". econstructor. eauto. eauto. Unshelve. all:todo "wf".
+Qed.
     
+Lemma leb_spect : forall x y : nat, BoolSpecSet (x <= y) (y < x) (x <=? y).
+Proof.
+  intros x y. destruct (x <=? y) eqn:E;
+  econstructor; destruct (Nat.leb_spec x y); lia.
+Qed.
+
+Lemma firstorder_args {Σ : global_env_ext} { mind cbody i n ui args u pandi oind} :
+  wf Σ ->
+  declared_constructor Σ (i, n) mind oind cbody ->
+  PCUICArities.typing_spine Σ [] (type_of_constructor mind cbody (i, n) ui) args (mkApps (tInd i u) pandi) ->
+  @firstorder_ind Σ (@firstorder_env Σ) i ui ->
+  firstorder_spine Σ [] (type_of_constructor mind cbody (i, n) ui) args (mkApps (tInd i u) pandi).
+Proof.
+  intros Hwf Hdecl Hspine  Hind. revert Hspine.
+  unshelve edestruct @declared_constructor_inv with (Hdecl := Hdecl); eauto. eapply weaken_env_prop_typing.
+
+  (* revert Hspine. *) unfold type_of_constructor.
+  erewrite cstr_eq. 2: eapply p.
+  rewrite <- it_mkProd_or_LetIn_app.
+  rewrite PCUICUnivSubst.subst_instance_it_mkProd_or_LetIn. 
+  rewrite PCUICSpine.subst0_it_mkProd_or_LetIn. intros Hspine.
+
+  match goal with
+   | [ |- firstorder_spine _ _ ?T _ _ ] =>
+  assert (@instantiated Σ [] T) as Hi end.
+  { clear Hspine. destruct Hdecl as [[d1 d3] d2]. pose proof d3 as Hdecl.
+    unfold firstorder_ind in Hind. 
+    rewrite d1 in Hind. solve_all. clear a.
+    eapply map_nth_error in d3.
+    rewrite nth_nth_error in H0.
+    rewrite d3 in H0.
+    unfold firstorder_oneind in H0.
+    solve_all.
+    eapply nth_error_all in H0. 2: eauto.
+    cbn in H0. unfold firstorder_con in H0. solve_all.
+    revert H0. cbn. unfold context. generalize ((subst_context (inds (inductive_mind i) ui (ind_bodies mind)) 0
+    (cstr_args cbody ++ ind_params mind)%list@[ui])). clear - Hdecl.
+    (* generalize conclusion to mkApps tInd args *)
+    intros c. induction c using PCUICInduction.ctx_length_rev_ind.
+    - unfold cstr_concl, cstr_concl_head.
+      autorewrite with substu subst. autorewrite with list.
+      rewrite PCUICInductives.subst_inds_concl_head. { cbn. eapply nth_error_Some. rewrite Hdecl. congruence. }
+      econstructor.
+    - intros Hall. eapply All_app in Hall as [Hall1 Hall2]. inv Hall2. destruct d. cbn in *.
+      rewrite it_mkProd_or_LetIn_app. cbn. destruct decl_body. 
+      + todo "letin".
+      + cbn. unfold firstorder_type in H0.
+        destruct ((PCUICAstUtils.decompose_app decl_type)) eqn:E.
+        * cbn in H0. destruct t; inv H0.
+          destruct ind. eapply PCUICAstUtils.decompose_app_inv in E as E'.
+          rewrite E'. econstructor.
+          -- admit.
+          -- intros. unfold PA.subst10.
+             rewrite PCUICLiftSubst.subst_it_mkProd_or_LetIn.
+             (* stability of firstorder_type under subst *) 
+             admit. }
+    revert Hi Hspine.
+    unfold cstr_concl, cstr_concl_head.
+    autorewrite with substu subst. autorewrite with list.
+    rewrite PCUICInductives.subst_inds_concl_head. { cbn. destruct Hdecl as [[d1 d2] d3]. eapply nth_error_Some. rewrite d2. congruence. }
+    match goal with [ |- context[mkApps _ ?args]] => generalize args end. 
+    intros args' Hi Spine. eapply typing_spine_arity_spine in Spine.
+    revert Hi Spine.  cbn.
+    remember (mkApps (tInd i u) pandi) as concl. revert args' concl Heqconcl.
+    induction 3; subst. (* 
+    match goal with [ |- context[it_mkProd_or_LetIn ?x ?y]] => generalize x end.
+
+     (* generalize conclusion to mkApps tInd args *)
+  (* eapply typing_spine_arity_spine in Hspine. *)
+  revert Hi Hspine.
+  generalize (type_of_constructor mind cbody (i, n) ui). *)
+  (* intros t. induction 2. *)
+  - econstructor; eauto. all:admit.
+  - inv Hi.
+    + econstructor; eauto. admit.
+    + eapply PCUICCanonicity.invert_cumul_prod_ind in e. eauto.
+  - todo "letin".
+  - inv Hi.
+    + admit.
+    + econstructor. 5: cbn; eauto. all: eauto. 3: eapply equality_refl. all: eauto. all: admit.      
 Admitted.
+
+Lemma firstorder_univs (Σ : global_env_ext) i n cbody ui u mind oind :
+  declared_constructor Σ (i, n) mind oind cbody ->
+   PCUICEquality.R_global_instance Σ.1 (eq_universe Σ) 
+   (eq_universe Σ) (ConstructRef i n)
+   (ind_npars mind + context_assumptions (cstr_args cbody)) ui u
+-> @firstorder_ind Σ (firstorder_env Σ) i ui -> @firstorder_ind Σ (firstorder_env Σ) i u.
+Proof.
+  intros Hdecl Heq H. destruct Hdecl as [[Hdecl1 Hdecl2] Hdecl3]. red in Hdecl1. cbn in *.
+  unfold firstorder_ind in *. unfold PCUICEnvironment.fst_ctx in *.
+  rewrite Hdecl1 in H |- *.
+  solve_all.
+
+  unfold firstorder_mutind in H0.
+  eapply map_nth_error in Hdecl2 as H1.
+  erewrite nth_nth_error in H0. setoid_rewrite H1 in H0.
+  clear H1.
+  eapply map_nth_error in Hdecl2 as H1.
+  erewrite nth_nth_error. setoid_rewrite H1.
+  clear H1.
   
-Lemma firstorder_value_spec Σ Γ t i u args mind :
-  wf_ext Σ -> wf_local Σ Γ ->
-   Σ ;;; Γ |- t : mkApps (tInd i u) args -> 
+  unfold firstorder_oneind in *.
+  solve_all.
+
+  unfold firstorder_con in *.
+  solve_all.
+  revert H0. generalize (cstr_args x ++ ind_params mind)%list, 0.
+  (* 
+  rewrite !PCUICUnivSubstitutionConv.subst_instance_app in H0 |- *.
+  rewrite <- !subst_context_app0 in H0 |- *.
+  eapply All_app in H0 as []. eapply All_app_inv.
+  - revert a0. *)
+  induction l as [ | a c IH] using rev_ind.
+  - econstructor.
+  - rewrite !PCUICUnivSubstitutionConv.subst_instance_app. cbn.
+    change ((c@[ui] ++ [a@[ui]]))%list with (app_context ([a@[ui]]) (c@[ui])).
+    change ((c@[u] ++ [a@[u]]))%list with (app_context ([a@[u]]) (c@[u])). intros len.
+    rewrite !PCUICLiftSubst.subst_context_app.
+    unfold subst_context at 1 3. cbn. intros Hall.
+    eapply All_app in Hall as []. eapply All_app_inv; eauto.
+    inv a1. cbn. econstructor. 2:econstructor.
+    destruct a. cbn in *.
+
+    unfold firstorder_type in *.
+    
+ (*    destruct (PCUICAstUtils.decompose_app (subst (inds (inductive_mind i) u (ind_bodies mind)) len decl_type)) as [L R] eqn:ELR.
+    (* eapply (f_equal (fun t : term * list term => t@[ui])) in ELR as ELR1.
+     *) eapply (f_equal (fun t : term * list term => t@[u])) in ELR as ELR2.
+    rewrite !PCUICUnivSubstitutionConv.subst_instance_decompose_app in ELR2.
+    autorewrite with substu in ELR2.  unfold subst_instance in ELR2 at 1. unfold subst_instance_instance in ELR2.  cbn in ELR2.
+    cbn in ELR.
+    (* destruct (PCUICAstUtils.decompose_app (decl_type@[ui])) as [L R] eqn:ELR. *)
+    erewrite PCUICSubstitution.decompose_app_subst. 2: eauto. cbn.
+      destruct decl_type; cbn in *; try congruence.
+    + destruct (len <=? n0) ; cbn in *; try congruence.
+      destruct (nth_error (inds (inductive_mind i) ui (ind_bodies mind))  (n0 - len)) eqn:E; cbn in *; try congruence.
+      eapply PCUICInductiveInversion.inds_nth_error in E as E'; destruct E' as [m ->]. cbn in H2.
+      eapply nth_error_Some_length in E.
+      rewrite inds_length in E.
+      erewrite <- inds_length in E.
+      eapply nth_error_Some' in E as [k E].
+      setoid_rewrite E. 
+      eapply PCUICInductiveInversion.inds_nth_error in E as E'; destruct E' as [m' ->]. cbn in *.
+      destruct plookup_env as [f | ] eqn:Eenv; try congruence.
+      admit.
+    + admit.
+      cbn in *.
+      subst.
+      unfold inds in *.
+      destruct (nth_error (inds (inductive_mind i) u (ind_bodies mind)) (n0 - len)); cbn in *; try congruence.
+    
+
+    
+
+  rewrite subst_context_app.
+  autorewrite with subst.
+
+  eapply All_nth_error in H0. 2: eauto. *)
+Admitted.
+
+
+
+
+  
+Lemma firstorder_value_spec Σ t i u args mind :
+  wf_ext Σ -> wf_local Σ [] ->
+   Σ ;;; [] |- t : mkApps (tInd i u) args -> 
    PCUICWcbvEval.value t -> 
   lookup_env Σ (i.(inductive_mind)) = Some (InductiveDecl mind) ->
-  @firstorder_ind Σ (firstorder_env Σ) i ->
-  firstorder_value Σ Γ t.
+  @firstorder_ind Σ (firstorder_env Σ) i u ->
+  firstorder_value Σ [] t.
 Proof.
   intros Hwf Hwfl Hty Hvalue.
   revert mind i u args Hty.
@@ -1638,12 +1839,15 @@ Proof.
       eapply PCUICSpine.typing_spine_strengthen in spine. 3: eauto. 
       2: eapply PCUICInductiveInversion.declared_constructor_valid_ty; eauto.
 
-      eapply firstorder_args in spine; eauto. clear - spine IH.
+      eapply firstorder_args in spine; eauto.
+      2:{ eapply R_global_instance_cstr_irrelevant in r. 2: eauto. now eapply firstorder_univs; eauto. }
+         
+      clear c0 c1 e1 e Hty.
       induction spine.
       * econstructor.
       * destruct d as [d1 d2]. inv IH.
-        econstructor; [ eauto | ].
-        eapply IHspine; eauto.
+        econstructor. 2:eapply IHspine; eauto. 2: now inv Hargs.
+        eapply H0; eauto. eapply d0.
     + exfalso. eapply (PCUICCanonicity.typing_cofix_coind (args := args')) in Hty.
       red in Hfo. unfold firstorder_ind in Hfo.
       rewrite Hlookup in Hfo.
@@ -1656,13 +1860,42 @@ Proof.
     destruct (nth_error mfix idx); auto.
     inversion E; subst; clear E.
     eapply nth_error_None. now eapply leb_complete. 
-Qed.  
+Qed.
+(* 
+Lemma wcbeval_red Σ t v :
+  wf_ext Σ ->
+  welltyped Σ [] t ->
+  red Σ [] t v ->
+  (forall t', red1 Σ [] v t' -> False) ->
+  exists u, squash(PCUICWcbvEval.eval Σ t u).
+Proof.
+  intros Hwf HT Hred Hval. pose proof (normalisation Σ Hwf _ _ HT).
+  induction H as [t H IH]. inversion Hred.
+  + subst. inv X.
+    * destruct (IH (PA.subst10 a b)) as [u Hu].
+      -- repeat econstructor.
+      -- admit.
+      -- eauto. 
+      -- eexists. 
+    * admit.
+    * admit.
+  + subst. admit. 
+  + subst. admit.
+  +
+  destruct (reducible Σ [] t) as [[t' Hred] | Hred].
+  - assert (cored Σ [] t' t) as Hcored. { econstructor. eauto. }
+    eapply IH in Hcored. 2: admit.
+    inversion Hred; subst.
+    + intros t''. 
+    exists u.
+ *)
+
   
 Lemma firstorder_erases_deterministic {Σ t t' i u args mind} H H2 : 
   Σ ;;; [] |- t : mkApps (tInd i u) args -> 
   PCUICWcbvEval.value t ->
   lookup_env Σ (i.(inductive_mind)) = Some (InductiveDecl mind) ->
-  @firstorder_ind Σ (firstorder_env Σ) i ->
+  @firstorder_ind Σ (firstorder_env Σ) i u ->
   erases Σ [] t t' ->
   t' = erase Σ H [] t H2.
 Proof.
