pcuic/theories/PCUICProgress.v
@@ -1,0 +1,517 @@
+(* Distributed under the terms of the MIT license. *)
+From MetaCoq.Template Require Import config utils.
+From MetaCoq.PCUIC Require Import PCUICTyping PCUICEquality PCUICAst PCUICAstUtils
+  PCUICWeakeningConv PCUICWeakeningTyp PCUICSubstitution PCUICGeneration PCUICArities
+  PCUICWcbvEval PCUICSR PCUICInversion
+  PCUICUnivSubstitutionConv PCUICUnivSubstitutionTyp
+  PCUICElimination PCUICSigmaCalculus PCUICContextConversion
+  PCUICUnivSubst PCUICWeakeningEnvConv PCUICWeakeningEnvTyp
+  PCUICCumulativity PCUICConfluence
+  PCUICInduction PCUICLiftSubst PCUICContexts PCUICSpine
+  PCUICConversion PCUICValidity PCUICInductives PCUICConversion
+  PCUICInductiveInversion PCUICNormal PCUICSafeLemmata
+  PCUICParallelReductionConfluence
+  PCUICWcbvEval PCUICClosed PCUICClosedTyp
+  PCUICReduction PCUICCSubst PCUICOnFreeVars PCUICWellScopedCumulativity PCUICCanonicity PCUICWcbvEval.
+  
+Local Existing Instance config.extraction_checker_flags.
+
+Inductive typing_spine_pred {cf : checker_flags} Σ (Γ : context) (P : forall t T (H : Σ ;;; Γ |- t : T), Type) : term -> list term -> term -> Type :=
+| type_spine_pred_nil ty ty' (* s s' *) :
+    isType Σ Γ ty ->
+    isType Σ Γ ty' ->
+    (* forall H : Σ ;;; Γ |- ty : tSort s,
+    P ty (tSort s) H ->
+    forall H' : Σ ;;; Γ |- ty' : tSort s',
+    P ty' (tSort s') H' ->
+     *) Σ ;;; Γ ⊢ ty ≤ ty' ->
+    typing_spine_pred Σ Γ P ty [] ty'
+
+| type_spine_pred_cons ty hd tl na A B B' s' :
+    isType Σ Γ ty ->
+    forall H' : Σ ;;; Γ |- tProd na A B : tSort s',
+    P (tProd na A B) (tSort s') H' ->
+    Σ ;;; Γ ⊢ ty ≤ tProd na A B ->
+    forall H : Σ ;;; Γ |- hd : A,
+    P hd A H ->
+    typing_spine_pred Σ Γ P (subst10 hd B) tl B' ->
+    typing_spine_pred Σ Γ P ty (hd :: tl) B'.    
+
+Section WfEnv.
+  Context {cf : checker_flags} {Σ : global_env_ext} {wfΣ : wf Σ}.
+
+  Lemma typing_spine_pred_strengthen {Γ P T args U} : 
+    typing_spine_pred Σ Γ P T args U ->
+    isType Σ Γ T ->
+    forall T', 
+    isType Σ Γ T' ->
+    Σ ;;; Γ ⊢ T' ≤ T ->
+    typing_spine_pred Σ Γ P T' args U.
+  Proof.
+    induction 1 in |- *; intros T' isTy redT.
+    - constructor; eauto. transitivity ty; auto.
+    - specialize IHX with (T' := (B {0 := hd})).
+      assert (isType Σ Γ (B {0 := hd})) as HH. {
+        clear p.
+        eapply inversion_Prod in H' as (? & ? & ? & ? & ?); tea.
+        eapply isType_subst. econstructor. econstructor. rewrite subst_empty; eauto.
+        econstructor; red; cbn; eauto. 
+      }
+      do 3 forward IHX by pcuic.
+      intros Hsub.
+      eapply type_spine_pred_cons; eauto.
+      etransitivity; eauto.
+  Qed.
+
+End WfEnv.
+
+Lemma inversion_mkApps {cf : checker_flags} {Σ} {wfΣ :  wf Σ.1} {Γ f u T} s :
+  forall (H : Σ ;;; Γ |- mkApps f u : T) (HT : Σ ;;; Γ |- T : tSort s),
+  { A : term & { Hf : Σ ;;; Γ |- f : A & {s' & {HA : Σ ;;; Γ |- A : tSort s' &
+   typing_size Hf <= typing_size H ×
+   typing_size HA <= max (typing_size H) (typing_size HT) ×
+  typing_spine_pred Σ Γ (fun x ty Hx => typing_size Hx <= typing_size H) A u T}}}}.
+Proof.
+  revert f T.
+  induction u; intros f T. simpl. intros.
+  { exists T, H, s, HT. intuition pcuic.
+    econstructor. eexists; eauto. eexists; eauto. eapply isType_equality_refl. eexists; eauto. }
+  intros Hf Ht. simpl in Hf.
+  specialize (IHu (tApp f a) T).
+  epose proof (IHu Hf) as (T' & H' & s' & H1 & H2 & H3 & H4); tea. 
+  edestruct @inversion_App_size with (H0 := H') as (na' & A' & B' & s_ & Hf' & Ha & HA & Hs1 & Hs2 & Hs3 & HA'''); tea.
+  exists (tProd na' A' B'). exists Hf'. exists s_. exists HA. 
+  split. rewrite <- H2. lia.
+  split. rewrite <- Nat.le_max_l, <- H2. lia.
+  
+  unshelve econstructor.
+  5: eauto. 1: eauto. 
+  3:eapply isType_equality_refl; eexists; eauto.
+  1: eexists; eauto.
+  1, 2: rewrite <- H2; lia.
+  eapply typing_spine_pred_strengthen; tea.
+  eexists; eauto. clear Hs3.
+  eapply inversion_Prod in HA as (? & ? & ? & ? & ?); tea.
+  eapply isType_subst. econstructor. econstructor. rewrite subst_empty; eauto.
+  econstructor; red; cbn; eauto.
+  Unshelve. eauto. 
+Qed.
+
+Lemma typing_ind_env_app_size `{cf : checker_flags} :
+forall (P : global_env_ext -> context -> term -> term -> Type)
+       (Pdecl := fun Σ Γ wfΓ t T tyT => P Σ Γ t T)
+       (PΓ : global_env_ext -> context -> Type),
+
+  (forall Σ (wfΣ : wf Σ.1)  (Γ : context) (wfΓ : wf_local Σ Γ), 
+       All_local_env_over typing Pdecl Σ Γ wfΓ -> PΓ Σ Γ) ->
+
+  (forall Σ (wfΣ : wf Σ.1) (Γ : context) (wfΓ : wf_local Σ Γ) (n : nat) decl,
+      nth_error Γ n = Some decl ->
+      PΓ Σ Γ ->
+      P Σ Γ (tRel n) (lift0 (S n) decl.(decl_type))) ->
+
+  (forall Σ (wfΣ : wf Σ.1) (Γ : context) (wfΓ : wf_local Σ Γ) (u : Universe.t),
+      PΓ Σ Γ ->
+      wf_universe Σ u ->
+      P Σ Γ (tSort u) (tSort (Universe.super u))) ->
+
+  (forall Σ (wfΣ : wf Σ.1) (Γ : context) (wfΓ : wf_local Σ Γ) (n : aname) (t b : term) (s1 s2 : Universe.t),
+      PΓ Σ Γ ->
+      Σ ;;; Γ |- t : tSort s1 ->
+      P Σ Γ t (tSort s1) ->
+      Σ ;;; Γ,, vass n t |- b : tSort s2 ->
+      P Σ (Γ,, vass n t) b (tSort s2) -> P Σ Γ (tProd n t b) (tSort (Universe.sort_of_product s1 s2))) ->
+
+  (forall Σ (wfΣ : wf Σ.1) (Γ : context) (wfΓ : wf_local Σ Γ) (n : aname) (t b : term)
+          (s1 : Universe.t) (bty : term),
+      PΓ Σ Γ ->
+      Σ ;;; Γ |- t : tSort s1 ->
+      P Σ Γ t (tSort s1) ->
+      Σ ;;; Γ,, vass n t |- b : bty -> P Σ (Γ,, vass n t) b bty -> P Σ Γ (tLambda n t b) (tProd n t bty)) ->
+
+  (forall Σ (wfΣ : wf Σ.1) (Γ : context) (wfΓ : wf_local Σ Γ) (n : aname) (b b_ty b' : term)
+          (s1 : Universe.t) (b'_ty : term),
+      PΓ Σ Γ ->
+      Σ ;;; Γ |- b_ty : tSort s1 ->
+      P Σ Γ b_ty (tSort s1) ->
+      Σ ;;; Γ |- b : b_ty ->
+      P Σ Γ b b_ty ->
+      Σ ;;; Γ,, vdef n b b_ty |- b' : b'_ty ->
+      P Σ (Γ,, vdef n b b_ty) b' b'_ty -> P Σ Γ (tLetIn n b b_ty b') (tLetIn n b b_ty b'_ty)) ->
+
+  (forall Σ (wfΣ : wf Σ.1) (Γ : context) (wfΓ : wf_local Σ Γ) (t : term) T B L s,
+      PΓ Σ Γ ->
+      Σ ;;; Γ |- T : tSort s -> P Σ Γ T (tSort s) ->
+      forall (Ht : Σ ;;; Γ |- t : T), P Σ Γ t T ->
+
+      (* Give a stronger induction hypothesis allowing to crawl under applications *)
+      (forall t' T' (Ht' : Σ ;;; Γ |- t' : T'), typing_size Ht' <= typing_size Ht -> P Σ Γ t' T') ->
+      typing_spine_pred Σ Γ (fun u ty H => Σ ;;; Γ |- u : ty × P Σ Γ u ty) T L B ->
+
+      P Σ Γ (mkApps t L) B) ->
+
+  (forall Σ (wfΣ : wf Σ.1) (Γ : context) (wfΓ : wf_local Σ Γ) cst u (decl : constant_body),
+      Forall_decls_typing P Σ.1 ->
+      PΓ Σ Γ ->
+      declared_constant Σ.1 cst decl ->
+      consistent_instance_ext Σ decl.(cst_universes) u ->
+      P Σ Γ (tConst cst u) (subst_instance u (cst_type decl))) ->
+
+  (forall Σ (wfΣ : wf Σ.1) (Γ : context) (wfΓ : wf_local Σ Γ) (ind : inductive) u
+        mdecl idecl (isdecl : declared_inductive Σ.1 ind mdecl idecl),
+      Forall_decls_typing P Σ.1 ->
+      PΓ Σ Γ ->
+      consistent_instance_ext Σ mdecl.(ind_universes) u ->
+      P Σ Γ (tInd ind u) (subst_instance u (ind_type idecl))) ->
+
+  (forall Σ (wfΣ : wf Σ.1) (Γ : context) (wfΓ : wf_local Σ Γ) (ind : inductive) (i : nat) u
+          mdecl idecl cdecl (isdecl : declared_constructor Σ.1 (ind, i) mdecl idecl cdecl),
+      Forall_decls_typing P Σ.1 ->
+      PΓ Σ Γ ->
+      consistent_instance_ext Σ mdecl.(ind_universes) u ->
+      P Σ Γ (tConstruct ind i u) (type_of_constructor mdecl cdecl (ind, i) u)) ->
+
+    (forall (Σ : global_env_ext) (wfΣ : wf Σ) (Γ : context) (wfΓ : wf_local Σ Γ),     
+     forall (ci : case_info) p c brs indices ps mdecl idecl
+       (isdecl : declared_inductive Σ.1 ci.(ci_ind) mdecl idecl),
+       Forall_decls_typing P Σ.1 -> 
+       PΓ Σ Γ ->
+       mdecl.(ind_npars) = ci.(ci_npar) ->
+       eq_context_upto_names p.(pcontext) (ind_predicate_context ci.(ci_ind) mdecl idecl) ->
+       let predctx := case_predicate_context ci.(ci_ind) mdecl idecl p in
+       wf_predicate mdecl idecl p ->
+       consistent_instance_ext Σ (ind_universes mdecl) p.(puinst) ->
+       wf_local Σ (Γ ,,, predctx) ->
+       forall pret : Σ ;;; Γ ,,, predctx |- p.(preturn) : tSort ps,
+       P Σ (Γ ,,, predctx) p.(preturn) (tSort ps) ->
+       PΓ Σ (Γ ,,, predctx) ->
+       is_allowed_elimination Σ ps idecl.(ind_kelim) ->
+       ctx_inst Σ Γ (p.(pparams) ++ indices)
+         (List.rev (subst_instance p.(puinst) (mdecl.(ind_params) ,,, idecl.(ind_indices)))) ->
+       PCUICTyping.ctx_inst P Σ Γ (p.(pparams) ++ indices) 
+         (List.rev (subst_instance p.(puinst) (mdecl.(ind_params) ,,, idecl.(ind_indices)))) ->
+       Σ ;;; Γ |- c : mkApps (tInd ci.(ci_ind) p.(puinst)) (p.(pparams) ++ indices) ->
+       P Σ Γ c (mkApps (tInd ci.(ci_ind) p.(puinst)) (p.(pparams) ++ indices)) ->
+       isCoFinite mdecl.(ind_finite) = false ->
+       let ptm := it_mkLambda_or_LetIn predctx p.(preturn) in
+       wf_branches idecl brs ->
+       All2i (fun i cdecl br =>
+         (eq_context_upto_names br.(bcontext) (cstr_branch_context ci mdecl cdecl)) ×
+         let brctxty := case_branch_type ci.(ci_ind) mdecl idecl p br ptm i cdecl in
+         (PΓ Σ (Γ ,,, brctxty.1) ×
+          (Σ ;;; Γ ,,, brctxty.1 |- br.(bbody) : brctxty.2) ×
+           (P Σ (Γ ,,, brctxty.1) br.(bbody) brctxty.2) ×
+           (Σ ;;; Γ ,,, brctxty.1 |- brctxty.2 : tSort ps) ×
+           (P Σ (Γ ,,, brctxty.1) brctxty.2 (tSort ps)))) 0 idecl.(ind_ctors) brs ->
+       P Σ Γ (tCase ci p c brs) (mkApps ptm (indices ++ [c]))) ->
+
+  (forall Σ (wfΣ : wf Σ.1) (Γ : context) (wfΓ : wf_local Σ Γ) (p : projection) (c : term) u
+        mdecl idecl cdecl pdecl (isdecl : declared_projection Σ.1 p mdecl idecl cdecl pdecl) args,
+      Forall_decls_typing P Σ.1 -> PΓ Σ Γ ->
+      Σ ;;; Γ |- c : mkApps (tInd (fst (fst p)) u) args ->
+      P Σ Γ c (mkApps (tInd (fst (fst p)) u) args) ->
+      #|args| = ind_npars mdecl ->
+      let ty := snd pdecl in P Σ Γ (tProj p c) (subst0 (c :: List.rev args) (subst_instance u ty))) ->
+
+  (forall Σ (wfΣ : wf Σ.1) (Γ : context) (wfΓ : wf_local Σ Γ) (mfix : list (def term)) (n : nat) decl,
+      let types := fix_context mfix in
+      fix_guard Σ Γ mfix ->
+      nth_error mfix n = Some decl ->
+      PΓ Σ (Γ ,,, types) ->
+      All (fun d => {s & (Σ ;;; Γ |- d.(dtype) : tSort s)%type * P Σ Γ d.(dtype) (tSort s)})%type mfix ->
+      All (fun d => (Σ ;;; Γ ,,, types |- d.(dbody) : lift0 #|types| d.(dtype))%type *
+          P Σ (Γ ,,, types) d.(dbody) (lift0 #|types| d.(dtype)))%type mfix ->
+      wf_fixpoint Σ.1 mfix ->
+      P Σ Γ (tFix mfix n) decl.(dtype)) ->
+
+  (forall Σ (wfΣ : wf Σ.1) (Γ : context) (wfΓ : wf_local Σ Γ) (mfix : list (def term)) (n : nat) decl,
+      let types := fix_context mfix in
+      cofix_guard Σ Γ mfix ->
+      nth_error mfix n = Some decl ->
+      PΓ Σ (Γ ,,, types) ->       
+      All (fun d => {s & (Σ ;;; Γ |- d.(dtype) : tSort s)%type * P Σ Γ d.(dtype) (tSort s)})%type mfix ->
+      All (fun d => (Σ ;;; Γ ,,, types |- d.(dbody) : lift0 #|types| d.(dtype))%type *
+          P Σ (Γ ,,, types) d.(dbody) (lift0 #|types| d.(dtype)))%type mfix ->
+      wf_cofixpoint Σ.1 mfix ->
+      P Σ Γ (tCoFix mfix n) decl.(dtype)) ->
+
+  (forall Σ (wfΣ : wf Σ.1) (Γ : context) (wfΓ : wf_local Σ Γ) (t A B : term) s,
+      PΓ Σ Γ ->
+      Σ ;;; Γ |- t : A ->
+      P Σ Γ t A ->
+      Σ ;;; Γ |- B : tSort s ->
+      P Σ Γ B (tSort s) ->
+      Σ ;;; Γ |- A <=s B ->
+      P Σ Γ t B) ->
+
+     env_prop P PΓ. 
+Proof.
+ intros P Pdecl PΓ.
+ intros XΓ X X0 X1 X2 X3 X4 X5 X6 X7 X8 X9 X10 X11 X12 Σ wfΣ Γ t T H.
+ eapply typing_ind_env_app_size; eauto. clear Σ wfΣ Γ t T H.
+ intros Σ wfΣ Γ wfΓ t na A B u s HΓ Hprod IHprod Ht IHt IH Hu IHu.
+ pose proof (mkApps_decompose_app t).
+ destruct (decompose_app t) as [t1 L].
+ subst. rename t1 into t. cbn in *.
+ replace (tApp (mkApps t L) u) with (mkApps t (L ++ [u])) by now rewrite mkApps_app.
+ 
+ pose proof (@inversion_mkApps cf) as Happs. specialize Happs with (H := Ht).
+ forward Happs; eauto.
+ destruct (Happs _ Hprod) as (A' & Hf & s' & HA & sz_f & sz_A & HL).
+ destruct @inversion_Prod_size with (H0 := Hprod) as (s1 & s2 & H1 & H2 & Hs1 & Hs2 & Hsub); [ eauto | ]. 
+ eapply X4. 6:eauto. all: eauto.
+ - eapply (IH _ _ HA). rewrite sz_A. todo "matthieu".
+ - intros. eapply (IH _ _ Ht'). rewrite H. exact sz_f.
+ - clear sz_A. induction L in A', Hf, (* HA, sz_A, *) Ht, HL, t, Hf, IH (*, s' *) |- *. 
+   + inversion HL; subst. inversion X13. econstructor. econstructor; eauto. eauto. eauto. eauto. eauto. eauto.
+     econstructor. 1,2: eapply isType_apply; eauto. eapply equality_refl.
+     eapply typing_closed_context; eauto. eapply type_is_open_term.
+     eapply type_App; eauto.
+   + cbn. inversion HL. subst. clear HL.
+     eapply inversion_Prod in H' as Hx; eauto. destruct Hx as (? & ? & ? & ? & ?).
+     econstructor.
+     7: unshelve eapply IHL.
+     now eauto. now eauto. now eauto. now eauto. now eauto. now eauto. 2:cbn in *; eauto.
+     eapply IH. econstructor; eauto. econstructor; eauto. now eapply cumulAlgo_cumulSpec in X14.
+     eauto.
+Qed.
+
+Lemma typing_ind_env `{cf : checker_flags} :
+  forall (P : global_env_ext -> context -> term -> term -> Type)
+         (Pdecl := fun Σ Γ wfΓ t T tyT => P Σ Γ t T)
+         (PΓ : global_env_ext -> context -> Type),
+
+    (forall Σ (wfΣ : wf Σ.1)  (Γ : context) (wfΓ : wf_local Σ Γ), 
+         All_local_env_over typing Pdecl Σ Γ wfΓ -> PΓ Σ Γ) ->
+
+    (forall Σ (wfΣ : wf Σ.1) (Γ : context) (wfΓ : wf_local Σ Γ) (n : nat) decl,
+        nth_error Γ n = Some decl ->
+        PΓ Σ Γ ->
+        P Σ Γ (tRel n) (lift0 (S n) decl.(decl_type))) ->
+
+    (forall Σ (wfΣ : wf Σ.1) (Γ : context) (wfΓ : wf_local Σ Γ) (u : Universe.t),
+        PΓ Σ Γ ->
+        wf_universe Σ u ->
+        P Σ Γ (tSort u) (tSort (Universe.super u))) ->
+
+    (forall Σ (wfΣ : wf Σ.1) (Γ : context) (wfΓ : wf_local Σ Γ) (n : aname) (t b : term) (s1 s2 : Universe.t),
+        PΓ Σ Γ ->
+        Σ ;;; Γ |- t : tSort s1 ->
+        P Σ Γ t (tSort s1) ->
+        Σ ;;; Γ,, vass n t |- b : tSort s2 ->
+        P Σ (Γ,, vass n t) b (tSort s2) -> P Σ Γ (tProd n t b) (tSort (Universe.sort_of_product s1 s2))) ->
+
+    (forall Σ (wfΣ : wf Σ.1) (Γ : context) (wfΓ : wf_local Σ Γ) (n : aname) (t b : term)
+            (s1 : Universe.t) (bty : term),
+        PΓ Σ Γ ->
+        Σ ;;; Γ |- t : tSort s1 ->
+        P Σ Γ t (tSort s1) ->
+        Σ ;;; Γ,, vass n t |- b : bty -> P Σ (Γ,, vass n t) b bty -> P Σ Γ (tLambda n t b) (tProd n t bty)) ->
+
+    (forall Σ (wfΣ : wf Σ.1) (Γ : context) (wfΓ : wf_local Σ Γ) (n : aname) (b b_ty b' : term)
+            (s1 : Universe.t) (b'_ty : term),
+        PΓ Σ Γ ->
+        Σ ;;; Γ |- b_ty : tSort s1 ->
+        P Σ Γ b_ty (tSort s1) ->
+        Σ ;;; Γ |- b : b_ty ->
+        P Σ Γ b b_ty ->
+        Σ ;;; Γ,, vdef n b b_ty |- b' : b'_ty ->
+        P Σ (Γ,, vdef n b b_ty) b' b'_ty -> P Σ Γ (tLetIn n b b_ty b') (tLetIn n b b_ty b'_ty)) ->
+
+    (forall Σ (wfΣ : wf Σ.1) (Γ : context) (wfΓ : wf_local Σ Γ) (t : term) T B L s,
+        PΓ Σ Γ ->
+        Σ ;;; Γ |- T : tSort s -> P Σ Γ T (tSort s) ->
+        forall (Ht : Σ ;;; Γ |- t : T), P Σ Γ t T -> 
+  
+        (* Give a stronger induction hypothesis allowing to crawl under applications *)
+        typing_spine_pred Σ Γ (fun u ty H => Σ ;;; Γ |- u : ty × P Σ Γ u ty) T L B ->
+  
+        P Σ Γ (mkApps t L) B) ->
+
+    (forall Σ (wfΣ : wf Σ.1) (Γ : context) (wfΓ : wf_local Σ Γ) cst u (decl : constant_body),
+        Forall_decls_typing P Σ.1 ->
+        PΓ Σ Γ ->
+        declared_constant Σ.1 cst decl ->
+        consistent_instance_ext Σ decl.(cst_universes) u ->
+        P Σ Γ (tConst cst u) (subst_instance u (cst_type decl))) ->
+
+    (forall Σ (wfΣ : wf Σ.1) (Γ : context) (wfΓ : wf_local Σ Γ) (ind : inductive) u
+          mdecl idecl (isdecl : declared_inductive Σ.1 ind mdecl idecl),
+        Forall_decls_typing P Σ.1 ->
+        PΓ Σ Γ ->
+        consistent_instance_ext Σ mdecl.(ind_universes) u ->
+        P Σ Γ (tInd ind u) (subst_instance u (ind_type idecl))) ->
+
+    (forall Σ (wfΣ : wf Σ.1) (Γ : context) (wfΓ : wf_local Σ Γ) (ind : inductive) (i : nat) u
+            mdecl idecl cdecl (isdecl : declared_constructor Σ.1 (ind, i) mdecl idecl cdecl),
+        Forall_decls_typing P Σ.1 ->
+        PΓ Σ Γ ->
+        consistent_instance_ext Σ mdecl.(ind_universes) u ->
+        P Σ Γ (tConstruct ind i u) (type_of_constructor mdecl cdecl (ind, i) u)) ->
+    
+    (forall (Σ : global_env_ext) (wfΣ : wf Σ) (Γ : context) (wfΓ : wf_local Σ Γ),     
+    forall (ci : case_info) p c brs indices ps mdecl idecl
+      (isdecl : declared_inductive Σ.1 ci.(ci_ind) mdecl idecl),
+      Forall_decls_typing P Σ.1 -> 
+      PΓ Σ Γ ->
+      mdecl.(ind_npars) = ci.(ci_npar) ->
+      eq_context_upto_names p.(pcontext) (ind_predicate_context ci.(ci_ind) mdecl idecl) ->
+      let predctx := case_predicate_context ci.(ci_ind) mdecl idecl p in
+      wf_predicate mdecl idecl p ->
+      consistent_instance_ext Σ (ind_universes mdecl) p.(puinst) ->
+      wf_local Σ (Γ ,,, predctx) ->
+      forall pret : Σ ;;; Γ ,,, predctx |- p.(preturn) : tSort ps,
+      P Σ (Γ ,,, predctx) p.(preturn) (tSort ps) ->
+      PΓ Σ (Γ ,,, predctx) ->
+      is_allowed_elimination Σ ps idecl.(ind_kelim) ->
+      PCUICTyping.ctx_inst typing Σ Γ (p.(pparams) ++ indices)
+        (List.rev (subst_instance p.(puinst) (mdecl.(ind_params) ,,, idecl.(ind_indices)))) ->
+      PCUICTyping.ctx_inst P Σ Γ (p.(pparams) ++ indices) 
+        (List.rev (subst_instance p.(puinst) (mdecl.(ind_params) ,,, idecl.(ind_indices)))) ->
+      Σ ;;; Γ |- c : mkApps (tInd ci.(ci_ind) p.(puinst)) (p.(pparams) ++ indices) ->
+      P Σ Γ c (mkApps (tInd ci.(ci_ind) p.(puinst)) (p.(pparams) ++ indices)) ->
+      isCoFinite mdecl.(ind_finite) = false ->
+      let ptm := it_mkLambda_or_LetIn predctx p.(preturn) in
+      wf_branches idecl brs ->
+      All2i (fun i cdecl br =>
+        (eq_context_upto_names br.(bcontext) (cstr_branch_context ci mdecl cdecl)) ×
+        let brctxty := case_branch_type ci.(ci_ind) mdecl idecl p br ptm i cdecl in
+        (PΓ Σ (Γ ,,, brctxty.1) ×
+          (Σ ;;; Γ ,,, brctxty.1 |- br.(bbody) : brctxty.2) ×
+          (P Σ (Γ ,,, brctxty.1) br.(bbody) brctxty.2) ×
+          (Σ ;;; Γ ,,, brctxty.1 |- brctxty.2 : tSort ps) ×
+          (P Σ (Γ ,,, brctxty.1) brctxty.2 (tSort ps)))) 0 idecl.(ind_ctors) brs ->
+      P Σ Γ (tCase ci p c brs) (mkApps ptm (indices ++ [c]))) ->
+      
+    (forall Σ (wfΣ : wf Σ.1) (Γ : context) (wfΓ : wf_local Σ Γ) (p : projection) (c : term) u
+          mdecl idecl cdecl pdecl (isdecl : declared_projection Σ.1 p mdecl idecl cdecl pdecl) args,
+        Forall_decls_typing P Σ.1 -> PΓ Σ Γ ->
+        Σ ;;; Γ |- c : mkApps (tInd (fst (fst p)) u) args ->
+        P Σ Γ c (mkApps (tInd (fst (fst p)) u) args) ->
+        #|args| = ind_npars mdecl ->
+        let ty := snd pdecl in P Σ Γ (tProj p c) (subst0 (c :: List.rev args) (subst_instance u ty))) ->
+
+    (forall Σ (wfΣ : wf Σ.1) (Γ : context) (wfΓ : wf_local Σ Γ) (mfix : list (def term)) (n : nat) decl,
+        let types := fix_context mfix in
+        fix_guard Σ Γ mfix ->
+        nth_error mfix n = Some decl ->
+        PΓ Σ (Γ ,,, types) ->
+        All (fun d => {s & (Σ ;;; Γ |- d.(dtype) : tSort s)%type * P Σ Γ d.(dtype) (tSort s)})%type mfix ->
+        All (fun d => (Σ ;;; Γ ,,, types |- d.(dbody) : lift0 #|types| d.(dtype))%type *
+            P Σ (Γ ,,, types) d.(dbody) (lift0 #|types| d.(dtype)))%type mfix ->
+        wf_fixpoint Σ.1 mfix ->
+        P Σ Γ (tFix mfix n) decl.(dtype)) ->
+
+    (forall Σ (wfΣ : wf Σ.1) (Γ : context) (wfΓ : wf_local Σ Γ) (mfix : list (def term)) (n : nat) decl,
+        let types := fix_context mfix in
+        cofix_guard Σ Γ mfix ->
+        nth_error mfix n = Some decl ->
+        PΓ Σ (Γ ,,, types) ->
+        All (fun d => {s & (Σ ;;; Γ |- d.(dtype) : tSort s)%type * P Σ Γ d.(dtype) (tSort s)})%type mfix ->
+        All (fun d => (Σ ;;; Γ ,,, types |- d.(dbody) : lift0 #|types| d.(dtype))%type *
+            P Σ (Γ ,,, types) d.(dbody) (lift0 #|types| d.(dtype)))%type mfix ->
+        wf_cofixpoint Σ.1 mfix ->
+        P Σ Γ (tCoFix mfix n) decl.(dtype)) ->
+
+    (forall Σ (wfΣ : wf Σ.1) (Γ : context) (wfΓ : wf_local Σ Γ) (t A B : term) s,
+        PΓ Σ Γ ->
+        Σ ;;; Γ |- t : A ->
+        P Σ Γ t A ->
+        Σ ;;; Γ |- B : tSort s ->
+        P Σ Γ B (tSort s) ->
+        Σ ;;; Γ |- A <=s B ->
+        P Σ Γ t B) ->
+
+       env_prop P PΓ.
+Proof.
+  intros P Pdecl PΓ; unfold env_prop.
+  intros XΓ X X0 X1 X2 X3 X4 X5 X6 X7 X8 X9 X10 X11 X12 Σ wfΣ Γ t T H.
+  apply typing_ind_env_app_size; eauto.
+Qed.
+
+Local Hint Constructors value red1 : wcbv.
+
+
+Definition axiom_free Σ :=
+  forall c decl, declared_constant Σ c decl -> cst_body decl <> None. (* TODO: consolidate with PCUICConsistency *)
+
+Lemma progress `{cf : checker_flags}: 
+  env_prop (fun Σ Γ t T => axiom_free Σ -> Γ = [] -> Σ ;;; Γ |- t : T -> {t' & red1 Σ t t'} + (value t))
+           (fun _ _ => True).
+Proof with eauto with wcbv; try congruence.
+  eapply typing_ind_env...
+  - intros Σ wfΣ Γ wfΓ n decl Hdecl _ Hax -> Hty.
+    destruct n; inv Hdecl.
+  - intros Σ wfΣ Γ _ n b b_ty b' s1 b'_ty _ Hb_ty IHb_ty Hb IHb Hb' IHb' Hax -> H.
+    destruct (IHb Hax eq_refl) as [ [t' IH] | IH]; eauto with wcbv.
+  - intros Σ wfΣ Γ _ t T B L s _ HT IHT Ht IHt HL Hax -> H.
+    induction HL in t, Ht, IHt |- *.
+    + cbn. eauto.
+    + cbn. eapply IHHL.
+      2:{ do 2 (econstructor; eauto). now eapply cumulAlgo_cumulSpec in e. }
+      intros _ Happ.
+      destruct (IHt Hax eq_refl Ht) as [[t' IH] | IH]; eauto with wcbv.
+      assert (Ht' : Σ ;;; [] |- t : tProd na A B) by (econstructor; eauto; now eapply cumulAlgo_cumulSpec in e).
+      destruct p0 as [_ [[t' Hstep] | Hval]]; eauto using red1.
+      inversion IH as [t' Hatom eq | | f args Hvals Hstuck ]; subst.
+      * destruct t; inv Hatom; eauto using red1.
+        -- eapply inversion_Sort in Ht' as (? & ? & Ht'); tea.
+           eapply equality_Sort_Prod_inv in Ht'; eauto.
+        -- eapply inversion_Prod in Ht' as (? & ? & ? & ? & Ht'); tea.
+           eapply equality_Sort_Prod_inv in Ht'; eauto.
+        -- right. eapply value_app with (l := [hd]); eauto.
+        -- right. eapply value_app with (l := [hd]); eauto.
+        -- destruct (isStuckFix (tFix mfix idx) [hd]) eqn:E.
+           ++ right. eapply value_stuck_fix with (args := [hd]); eauto.
+           ++ cbn in E. eapply inversion_Fix in Ht' as ([] & ? & Efix & ? & ? & ?); eauto.
+              unfold cunfold_fix in E. rewrite Efix in E. cbn in *.
+              destruct rarg; inv E.
+              left. eexists. eapply red_fix with (argsv := []). (* TODO: red_fix rule is broken *)
+        -- todo "cofix".
+      * replace (tApp (mkApps t0 l) hd) with (mkApps t0 (l ++ [hd])) by now rewrite mkApps_app.
+        right. eapply value_app; eauto using All_app_inv.
+      * replace (tApp (mkApps f args) hd) with (mkApps f (args ++ [hd])) by now rewrite mkApps_app.
+        unfold isStuckFix in Hstuck. destruct f; try now inv Hstuck.
+        eapply PCUICValidity.inversion_mkApps in Ht' as (? & Hf & ?).
+        eapply inversion_Fix in Hf as ([] & ? & Efix & ? & ? & ?); eauto.
+        destruct (isStuckFix (tFix mfix idx) (args ++ [hd])) eqn:E.
+        ++ right. eapply value_stuck_fix; eauto using All_app_inv.
+        ++ cbn in E. unfold cunfold_fix in E. rewrite Efix in E. cbn in *.
+           left. eexists. rewrite mkApps_app. cbn. eapply red_fix. (* TODO: red_fix rule is broken *)
+  - intros Σ wf Γ _ cst u decl Hdecls _ Hdecl Hcons Hax -> H.
+    destruct (decl.(cst_body)) as [body | ] eqn:E.
+    + eauto with wcbv.
+    + red in Hax. eapply Hax in E; eauto.
+  - intros Σ wfΣ Γ _ ci p c brs indices ps mdecl idecl Hidecl Hforall _ Heq Heq_context predctx Hwfpred Hcon Hwfl Hreturn IHreturn _.
+    intros Helim Hinst Hctxinst Hc IHc Hcof ptm Hwfbranches Hall Hax -> H.
+    specialize (IHc Hax eq_refl) as [[t' IH] | IH]; eauto with wcbv.
+    eapply PCUICCanonicity.value_canonical in IH; eauto.
+    unfold head in IH.
+    rewrite (PCUICInduction.mkApps_decompose_app c) in H, Hc |- *.
+    destruct (decompose_app c) as [h l]. clear c.
+    cbn - [decompose_app] in *.
+    destruct h; inv IH.
+    + eapply invert_Case_Construct in H as H_; sq; eauto. destruct H_ as (Eq & H_); subst.
+      left.
+      destruct (nth_error brs n) as [br | ] eqn:E.
+      2:{ exfalso. firstorder congruence. }
+      assert (#|l| = ci_npar ci + context_assumptions (bcontext br)) as Hl by firstorder congruence.
+      clear H_. eapply Construct_Ind_ind_eq' in Hc as (? & ? & ? & ? & _); eauto.
+      eexists. eapply red_iota; eauto.
+    + todo "cofix".
+  - intros Σ wfΣ Γ _ ((i, pars), arg) c u mdecl idecl cdecl pdecl Hcon args Hargs _ Hc IHc
+           Hlen ty Hax -> H.
+    destruct (IHc Hax eq_refl) as [[t' IH] | IH]; eauto with wcbv; clear IHc.
+    eapply PCUICCanonicity.value_canonical in IH; eauto.
+    unfold head in IH.
+    rewrite (PCUICInduction.mkApps_decompose_app c) in H, Hc |- *.
+    destruct (decompose_app c) as [h l]. clear c.
+    cbn - [decompose_app] in *.
+    destruct h; inv IH.
+    + red in Hcon. cbn in *.
+      eapply invert_Proj_Construct in H as H_; sq; eauto. destruct H_ as (-> & -> & Hl).
+      left. eapply nth_error_Some' in Hl as [x Hx].
+      eauto with wcbv.
+    + todo "cofix". 
+    Unshelve. all: todo "shelved".
+Qed.
