template-coq/theories/EnvironmentTyping.v
@@ -1,4 +1,4 @@
-is(* Distributed under the terms of the MIT license. *)
+(* Distributed under the terms of the MIT license. *)
 From MetaCoq.Template Require Import config utils BasicAst Universes Environment.
 From Equations Require Import Equations.
 
